theories/Utils/Arith.v
@@ -2,9 +2,20 @@ From Coq Require Import
   Lia.
 Import PeanoNat.Nat.
 
+Theorem plus_reg_r : forall n m p : nat, n + p = m + p -> n = m.
+Proof.
+  intros n m p.
+  induction p as [|p IHp].
+  + repeat rewrite add_0_r; trivial.
+  + repeat rewrite <- plus_n_Sm.
+    intro eq.
+    injection eq as eq2.
+    apply IHp.
+    exact eq2.
+Qed.
+
 Definition lt_sub:
   forall {n m}, n < m -> {p : nat | m = p + n /\ 0 < p}.
-  Proof.  
     intros n m.
     generalize dependent n.
     induction m as [|m IHm]; intros n lnm. 
@@ -16,24 +27,23 @@ Definition lt_sub:
         destruct (IHm n lnm).
         exists x.
         lia.
-  Defined.
+Defined.
 
-  Definition le_sub:
+Definition le_sub:
   forall {n m}, n <= m -> {p : nat | m = p + n /\ 0 <= p}.
-  Proof.  
-    intros n m.
-    generalize dependent n.
-    induction m as [|m IHm]; intros n lnm. 
-    - exists 0.
+  intros n m.
+  generalize dependent n.
+  induction m as [|m IHm]; intros n lnm. 
+  - exists 0.
+    lia.
+  - destruct n as [|n].
+    + exists (S m).
       lia.
-    - destruct n as [|n].
-      + exists (S m).
-        lia.
-      + apply Le.le_S_n in lnm.
-        destruct (IHm n lnm).
-        exists x.
-        lia.
-  Defined.
+    + apply Le.le_S_n in lnm.
+      destruct (IHm n lnm).
+      exists x.
+      lia.
+Defined.
 
 (* Ceiling log base 2 function *)
 Definition clog2 (x : nat) : nat := 
